\documentclass{article}
\title{Homework 1}
\author{Jonathan Kalsky}
\date{Jan. 21 2026}

\begin{document}
\maketitle
\vspace{1cm}
\tableofcontents
\vspace{1cm}
\hrulefill
\vspace{1cm}

%Question 1:
\section{Write the truth table for $(p \land q) \land \lnot p$ :}

\begin{center}
    
    \begin{tabular}{| c | c | c |}
        \hline
        p & q & $(p \land q) \land \lnot p$\\
        \hline
        T & T & F\\
        T & F & F\\
        F & T & F\\
        F & F & F\\
        \hline
    \end{tabular}

\end{center}

%Question 2:
% \vspace{0.5cm}
% \bigskip
\section{Write the truth table for $\lnot p \land q \lor r \land \lnot p$}

$$
\begin{array}{|c|c|c|c|}
\hline
p & q & r & \lnot p \land q \lor r \land \lnot p \\
\hline
T & T & F & F\\
T & F & F & F\\
F & T & F & T\\
F & F & F & F\\
T & T & T & F\\
T & F & T & F\\
F & T & T & T\\
F & F & T & T\\
\hline
\end{array}
$$

%Question 3:
\section{Write the truth table for $(p \to q) \land (q \to r)$}
$$
    \begin{array}{|c|c|c|c|}
        \hline
        p & q & r & (p \to q) \land (q \to r) \\
        \hline
        F & F & F & T \\
        F & F & T & T\\
        F & T & F & F\\
        F & T & T & T\\
        T & F & F & F\\
        T & F & T & F\\
        T & T & F & F\\
        T & T & T & T\\
        \hline
    \end{array}
$$

%Question 4:
\section{Write the truth table for: $p \to q \to r$}
$$
\begin{array}{|c|c|c|c|}
    \hline
    p & q & r & p \to q \to r\\
    \hline
    F & F & F & T \\
    F & F & T & T\\
    F & T & F & T\\
    F & T & T & T\\
    T & F & F & T\\
    T & F & T & T\\
    T & T & F & F\\
    T & T & T & T\\
    \hline
\end{array}
$$

%Question 5:
\newpage
\noindent
\section{Use the theorems of logical equivalence to prove the following logical equivalence: $(p \land \lnot q) \lor p \equiv p$}

Distributive Law
$$
(p \land \lnot q) \lor p \equiv (p \lor p) \land (p \lor \lnot q)
$$
Idempotent Law
$$
(p \lor p) \equiv p
$$
Substitute
$$
(p \land \lnot q) \lor p \equiv p \land (p \lor \lnot q)
$$
Absorption Law
$$
p \land (p \lor \lnot q) \equiv p
$$
Finally
$$
(p \land \lnot q) \lor p \equiv p
$$

\section{Use the theorems of logical equivalence to prove the following logical equivalence: $p \land (\lnot q \lor p) \equiv p$}
Absorption Law
$$
p \land (\lnot q \lor p) \equiv p
$$
\end{document}

